CertiGC/verif_forward_remset.v
@@ -89,16 +89,15 @@ Proof.
                         (sublist 0 n (Znth (Z.of_nat from) rh)) (g, h, rh, rmst);
                         0 <= n <= total_size h from - available_size h from)
                   LOCAL (temp _q
-                           (offset_val (WORD_SIZE *
-                                          (available_space (nth_space h' from) + n))
+                           (offset_val (WORD_SIZE * (available_size h' from + n))
                               (space_start (nth_space h' from)));
                          temp _from_rem_limit
-                           (offset_val (WORD_SIZE * total_space (nth_space h' from))
+                           (offset_val (WORD_SIZE * total_size h' from)
                               (space_start (nth_space h' from)));
                          temp _from_limit
-                           (offset_val (WORD_SIZE * available_space (nth_space h' from))
+                           (offset_val (WORD_SIZE * available_size h' from)
                               (space_start (nth_space h' from)));
-                         temp _from_start (space_start (nth_space h from));
+                         temp _from_start (space_start (nth_space h' from));
                          temp _from (space_address hp from);
                          temp _to (space_address hp to);
                          temp _next (heap_next_address hp to))
@@ -163,16 +162,16 @@ Proof.
       * change (Tpointer Tvoid {| attr_volatile := false; attr_alignas := Some 3%N |})
           with int_or_ptr_type in *. remember (space_start (nth_space h' from)) as vs.
         remember (offset_val _ vs) as va.
-        remember (offset_val (WORD_SIZE * total_space (nth_space h' from)) vs) as vt.
+        remember (offset_val (WORD_SIZE * total_size h' from) vs) as vt.
         assert (Hva: isptr va) by now subst va; apply isptr_offset_val'.
         assert (Hvt: isptr vt) by now subst vt; apply isptr_offset_val'.
         Transparent denote_tc_test_eq. unfold denote_tc_test_eq. destruct va; try contradiction.
         destruct vt; try contradiction. rewrite Heqva, Heqvt. unfold test_eq_ptrs.
         rewrite sameblock_offset_val by assumption. unfold heap_rep. apply andp_right.
         -- sep_apply (graph_and_heap_remset_weak_valid_ptr g' h' rh' from
-                        (WORD_SIZE * (available_space (nth_space h' from) + n))). entailer !!.
+                        (WORD_SIZE * (available_size h' from + n))). entailer !!.
         -- sep_apply (graph_and_heap_remset_weak_valid_ptr g' h' rh' from
-                        (WORD_SIZE * (total_space (nth_space h' from)))). 2: entailer !!.
+                        (WORD_SIZE * (total_size h' from))). 2: entailer !!.
            pose proof total_space_tight_range (nth_space h' from). unfold total_size, WORD_SIZE. lia.
       * change (Tpointer tvoid {| attr_volatile := false; attr_alignas := Some 3%N |})
           with int_or_ptr_type in *. freeze [0; 1; 2; 3; 4] FR. rename H into Hneq.
@@ -189,8 +188,7 @@ Proof.
         remember (total_size h' _ - available_size h' _) as rh_size.
         remember (map (remset_item_val g') (nth_remset_space rh' from)) as rh_value.
         assert (Hrhs: rh_size = Zlength rh_value). {
-          subst. rewrite Zlength_map. eapply rhhc_rssc with (gen := from) in Hrhhc'; eauto. hnf in Hrhhc'.
-          destruct (Val.eq _ _). 1: rewrite e in Hptrf'; contradiction. symmetry. assumption. }
+          subst. rewrite Zlength_map. symmetry. eapply rhhc_rssc_len; eassumption. }
         assert (Hrdb: readable_share (space_sh (nth_space h' from))). {
           rewrite <- Hshf'. apply writable_readable, generation_share_writable. }
         assert (Hprt: isptr (Znth n rh_value)). {
@@ -264,14 +262,15 @@ Proof.
           rewrite sizeof_tarray_int_or_ptr; [Intros; cancel | unfold available_size].
           destruct (available_space_tight_range (nth_space h' from)). assumption. }
         subst rh_value. remember (Znth n (map _ _)) as rh_value. rewrite Znth_map in Heqrh_value.
-        remember (Znth n (nth_remset_space rh' from)) as item. destruct item.
-        -- simpl in Heqrh_value. subst rh_value. rewrite Zlength_map in Hrhs.
-           assert (Hinv: In v (map extract_address rmst')). {
-             hnf in Hrrhc'. rewrite Forall_forall_Znth in Hrrhc'.
-             assert (0 <= (Z.of_nat from) < Zlength rh') by (eapply gen_range_remset_heap; eassumption).
-             specialize (Hrrhc' _ H). hnf in Hrrhc'. rewrite Forall_forall_Znth in Hrrhc'.
-             rewrite <- nth_remset_space_Znth in Hrrhc'. rewrite Hrhs in Hnrange.
-             specialize (Hrrhc' _ Hnrange). rewrite <- Heqitem in Hrrhc'. simpl in Hrrhc'. assumption. }
+        2: rewrite Zlength_map in Hrhs; rewrite <- Hrhs; assumption.
+        remember (Znth n (nth_remset_space rh' from)) as item. rewrite Zlength_map in Hrhs.
+        assert (Hric: remset_item_compatible g' from rmst' item). {
+          hnf in Hrrhc'. rewrite Forall_forall_Znth in Hrrhc'.
+          assert (0 <= (Z.of_nat from) < Zlength rh') by (eapply gen_range_remset_heap; eassumption).
+          specialize (Hrrhc' _ H). hnf in Hrrhc'. rewrite Forall_forall_Znth in Hrrhc'.
+          rewrite <- nth_remset_space_Znth in Hrrhc'. rewrite Hrhs in Hnrange.
+          specialize (Hrrhc' _ Hnrange). rewrite <- Heqitem in Hrrhc'. assumption. } destruct item.
+        -- simpl in Heqrh_value. subst rh_value. simpl in Hric. rename Hric into Hinv.
            gather_SEP (graph_rep _) (heap_unused_rep _) (remset_rep _ _ _). rewrite <- HeqP.
            replace_SEP 0 ((weak_derives P (memory_block fsh fn fp * TT) && emp) * P) by
              (entailer !!; assumption). Intros.
@@ -284,7 +283,25 @@ Proof.
            forward_call (fsh, fp, fn, v, P). Intros vret. destruct vret as [Hvin | Hvnot].
            ++ subst. sep_apply (v_in_range_graph_remset_rep_FF sh g' h' rmst' from v).
               assert_PROP False by entailer !. contradiction.
-           ++ forward_if True. 2: contradiction.
+           ++ forward_if (EX g3: LGraph, EX h3: heap, EX rh3: remset_heap, EX rmst3: remset,
+                          PROP ((g3, h3, rh3, rmst3) = forward_remset_item from to
+                                                         (g', h', rh', rmst') (RemSetExterior v))
+                          LOCAL (temp _q
+                                   (offset_val (WORD_SIZE * (available_size h' from + n))
+                                      (space_start (nth_space h' from)));
+                                 temp _from_rem_limit
+                                   (offset_val (WORD_SIZE * total_size h' from)
+                                      (space_start (nth_space h' from)));
+                                 temp _from_limit
+                                   (offset_val (WORD_SIZE * available_size h' from)
+                                      (space_start (nth_space h' from)));
+                                 temp _from_start (space_start (nth_space h' from));
+                                 temp _from (space_address hp from);
+                                 temp _to (space_address hp to);
+                                 temp _next (heap_next_address hp to))
+                  SEP (heap_rep sh h3 hp; all_string_constants rsh gv; outlier_rep outlier;
+                       graph_rep g3; heap_remset_rep g3 h3 rh3; remset_rep sh g3 rmst3)).
+              2: contradiction.
               ** subst P. clear H Pweak Hweakp Hgenat. Intros.
                  gather_SEP (heap_struct_rep _ _ _) (heap_unused_rep _). fold (heap_rep sh h' hp).
                  pose proof get_remset_ext_In v rmst' Hinv as Hrin.
@@ -342,5 +359,223 @@ Proof.
                  unlocalize [heap_struct_rep sh
                                (map space_quad (spaces (incr_remset_heap h2 (Z.of_nat to)))) hp].
                  1: pose proof gen_range _ _ _ Hghc Hghgt; apply heap_rem_ramif; lia. thaw FR.
-                 (* forward. *)
-Abort.
+                 assert (Htemp: heap_remset_rep g' h' rh' = heap_remset_rep g2 h2 rh') by
+                   (eapply fgh_heap_remset_rep; eassumption). rewrite Htemp. clear Htemp.
+                 assert (Htemp: 0 < remset_gen_size h' from - n). {
+                   unfold remset_gen_size. rewrite <- Heqgn, <- Heqrh_size. lia. }
+                 assert (Hgesc2: general_enough_space_to_copy g2 h2 from to
+                                   (remset_gen_size h' from - n)) by
+                   (eapply forward_graph_and_heap_O_gestc; try eassumption; lia).
+                 assert (Hulta: used_space (nth_space h2 to) < available_space (nth_space h2 to)). {
+                   red in Hgesc2. pose proof unmarked_gen_size_nonneg g2 from.
+                   unfold rest_gen_size in Hgesc2. lia. } clear Htemp Hgesc2.
+                 sep_apply (heap_unused_rep_incr g2 h2 to). Intros.
+                 gather_SEP (heap_struct_rep _ _ _) (heap_unused_rep _).
+                 replace_SEP 0 (heap_rep sh (incr_remset_heap h2 (Z.of_nat to)) hp) by
+                   (unfold heap_rep; entailer !!).
+                 pose proof generation_share_writable (nth_gen g2 to) as Hws. rewrite Hsht2 in Hws.
+                 gather_SEP (data_at_ _ _ _) (heap_remset_rep _ _ _). Intros.
+                 assert (Hrhhc2: remset_heap_and_heap_compatible rh' h2). {
+                   apply heap_relation_rhhc with h'; auto.
+                   pose proof heaprel_forward_graph_and_heap from to O (remset_ext2forward_t rext) g' h'.
+                   rewrite <- Hfgh in H. simpl in H. assumption. }
+                 assert ((g2, incr_remset_heap h2 (Z.of_nat to),
+                           upd_remset_heap (RemSetExterior v) rh' to,
+                           upd_remset from to g' (RemSetExterior v) rmst') =
+                           forward_remset_item from to (g', h', rh', rmst') (RemSetExterior v)). {
+                   simpl. rewrite get_remset_ext_fact with (Hin := Hinv). rewrite <- Heqrext.
+                   rewrite <- Hfgh. reflexivity. }
+                 forward.
+                 Exists g2 (incr_remset_heap h2 (Z.of_nat to))
+                   (upd_remset_heap (RemSetExterior v) rh' to)
+                   (upd_remset from to g' (RemSetExterior v) rmst'). unfold limit_address.
+                 clear Heqfp. rewrite <- Hgens in Haddrf'.
+                 entailer !!. 2: sep_apply remset_rep_upd_ext; auto.
+                 rewrite Haddrf'; unfold available_size; f_equal. lia.
+              ** Intros g3 h3 rh3 rmst3. rename H into Hfri. forward.
+                 Exists (n + 1) g3 h3 rh3 rmst3.
+                 pose proof fri_available_size _ _ _ _ _ _ _ _ _ _ _ Hftneq Hfri as Hfas.
+                 pose proof fri_total_size _ _ _ _ _ _ _ _ _ _ _ Hftneq Hfri as Hfts.
+                 assert (Hfss: space_start (nth_space h3 from) = space_start (nth_space h' from)). {
+                   apply forward_remset_item_whr in Hfri. hnf in Hfri. destruct Hfri as [Hfri _].
+                   rewrite Hfri. reflexivity. } rewrite Hfas, Hfts, Hfss.
+                 assert (Hrheq: nth_remset_space rh from = nth_remset_space rh' from). {
+                       eapply fri_fold_rh_same; eauto. pose proof gen_range_heap _ _ _ Hghc Hghgt.
+                       clear -H Hrhhc. hnf in Hrhhc. rewrite Forall2_forall_Znth in Hrhhc. lia. }
+                 entailer !!. split; [|split].
+                 --- rewrite <- nth_remset_space_Znth in *.
+                     rewrite Hrheq in *. rewrite sublist_last_1 by lia.
+                     rewrite fold_left_app, <- Hfric. auto. rewrite <- Heqitem.
+                     Opaque forward_remset_item. simpl. Transparent forward_remset_item. assumption.
+                 --- rewrite Hrhs, <- Hrheq in Hnrange.
+                     rewrite (rhhc_rssc_len g h rh) in Hnrange; auto. lia.
+                 --- f_equal. simpl. unfold WORD_SIZE. lia.
+        -- simpl in Heqrh_value. destruct i as [v pos]. subst rh_value. simpl in Hric.
+           destruct Hric as [Hghv' [Hpos Hvfrom]].
+           gather_SEP (graph_rep _) (heap_unused_rep _) (remset_rep _ _ _). rewrite <- HeqP.
+           replace_SEP 0 ((weak_derives P (memory_block fsh fn fp * TT) && emp) * P) by
+             (entailer !!; assumption). Intros.
+           assert (P |-- (weak_derives P (valid_pointer (offset_val (pos * WORD_SIZE)
+                                                           (vertex_address g' v)) * TT) && emp) * P)
+             as Hweakp. {
+             subst. cancel. apply andp_right. 2: cancel.
+             assert (HS: emp |-- TT) by entailer; sep_apply HS; clear HS. apply derives_weak.
+             sep_apply (graph_rep_interiro_vptr g' v pos). cancel. }
+           replace_SEP 1 ((weak_derives P (valid_pointer (offset_val (pos * WORD_SIZE)
+                                                            (vertex_address g' v)) * TT) && emp) * P) by
+             (entailer !!; assumption). Intros.
+           forward_call (fsh, fp, fn, (offset_val (pos * WORD_SIZE)
+                                         (vertex_address g' v)), P). Intros vret.
+           forward_if (EX g3: LGraph, EX h3: heap, EX rh3: remset_heap, EX rmst3: remset,
+                       PROP ((g3, h3, rh3, rmst3) =
+                               forward_remset_item from to
+                                 (g', h', rh', rmst') (RemSetInterior (InteriorVertexPos v pos)))
+                       LOCAL (temp _q
+                                (offset_val (WORD_SIZE * (available_size h' from + n))
+                                   (space_start (nth_space h' from)));
+                              temp _from_rem_limit
+                                (offset_val (WORD_SIZE * total_size h' from)
+                                   (space_start (nth_space h' from)));
+                              temp _from_limit
+                                (offset_val (WORD_SIZE * available_size h' from)
+                                   (space_start (nth_space h' from)));
+                              temp _from_start (space_start (nth_space h' from));
+                              temp _from (space_address hp from);
+                              temp _to (space_address hp to);
+                              temp _next (heap_next_address hp to))
+                       SEP (heap_rep sh h3 hp; all_string_constants rsh gv; outlier_rep outlier;
+                            graph_rep g3; heap_remset_rep g3 h3 rh3; remset_rep sh g3 rmst3)).
+           ++ destruct vret as [Hvin | Hvnot].
+              1: fold Int.one in H; exfalso; revert H; apply Int.one_not_zero. subst P.
+              clear Pweak Hweakp H. Intros.
+              sep_apply (graph_and_heap_rest_v_in_range_iff_offset g' h' from v pos). Intros.
+              rewrite <- Hgens, Heqfn, Heqgn, H in Hvnot. clear H. specialize (Hvfrom Hvnot).
+              gather_SEP (heap_struct_rep _ _ _) (heap_unused_rep _). fold (heap_rep sh h' hp).
+              remember (FwdPntIntr (InteriorVertexPos v pos)) as fpi.
+              assert (Hpam: forward_p_addr_match fpi None) by (subst; simpl; auto).
+              assert (Hpc: forward_p_compatible fpi outlier g' from). {
+                subst fpi. simpl. destruct Hvfrom. split; auto. }
+              assert (Hfpr: forward_p_rep sh fpi None g' = emp) by (subst fpi; simpl; reflexivity).
+              rewrite <- (emp_sepcon (heap_rep sh h' hp)). Intros. rewrite <- Hfpr.
+              assert (Hfpa: forward_p_address fpi None g' =
+                              offset_val (pos * WORD_SIZE) (vertex_address g' v)). {
+                subst fpi. simpl. f_equal; lia. } rewrite <- Hfpa.
+              rewrite <- Hgens, Heqfn, Heqgn. fold (limit_address g' h' from).
+              forward_call (rsh, sh, gv, g', h', hp, outlier, from, to, 0, fpi, @None val).
+              Intros vret. destruct vret as [g2 h2]. rename H into Hfgh. clear Hpam Hpc Hfpr Hfpa.
+              subst fpi. simpl in Hfgh. simpl. remember (field2forward _) as ft.
+              gather_SEP (all_string_constants _ _) emp. rewrite sepcon_emp.
+              erewrite fgh_O_remset_rep_int_eq; eauto. 2: eapply remset_compatible_weakened; eassumption.
+              assert (Hftc: forward_t_compatible ft g'). {
+                subst ft; apply vertex_pos_forward_t_compatible; assumption. }
+              assert (Hghc2: graph_heap_compatible g2 h2). {
+                eapply forward_graph_and_heap_O_ghc with (g := g'); eauto. }
+              assert (Hghgt2: graph_has_gen g2 to). {
+                pose proof fr_forward_graph_and_heap from to O ft g' h'.
+                rewrite <- Hfgh in H. simpl in H. erewrite <- fr_graph_has_gen; eassumption. }
+              assert (Hgsc: generation_space_compatible g2 (to, nth_gen g2 to, nth_space h2 to)) by
+                (apply gt_gs_compatible; assumption). destruct Hgsc as [Haddrt2 [Hsht2 Hsizet2]].
+              assert (Hptrt2: isptr (space_start (nth_space h2 to))) by
+                (rewrite <- Haddrt2; apply start_isptr). unfold heap_rep. Intros.
+              freeze [0; 1; 2; 4; 5; 6] FR.
+              localize [space_struct_rep sh hp h2 to].
+              unfold space_struct_rep, space_quad.
+              forward.
+              forward.
+              simpl force_val. rewrite sem_sub_pi_available_space_minus; auto.
+              forward.
+              replace_SEP 0 (space_struct_rep sh hp (incr_remset_heap h2 (Z.of_nat to)) to). {
+                entailer !!. unfold space_struct_rep, space_quad.
+                rewrite irh_used_space, irh_space_start, irh_total_space, irh_available_space_same.
+                - cancel.
+                - eapply gen_range_heap; eassumption.
+                - assert (0 < remset_gen_size h' from - n) by (unfold remset_gen_size; lia).
+                  eapply forward_graph_and_heap_O_gestc in Hfgh; eauto. 2: lia. clear -Hfgh H.
+                  red in Hfgh. pose proof unmarked_gen_size_nonneg g2 from.
+                  unfold rest_gen_size in Hfgh. lia. }
+              unlocalize [heap_struct_rep sh
+                            (map space_quad (spaces (incr_remset_heap h2 (Z.of_nat to)))) hp].
+              1: pose proof gen_range _ _ _ Hghc Hghgt; apply heap_rem_ramif; lia. thaw FR.
+              assert (Htemp: heap_remset_rep g' h' rh' = heap_remset_rep g2 h2 rh'). {
+                eapply (fgh_heap_remset_rep _ _ _ from _); eassumption. } rewrite Htemp. clear Htemp.
+              assert (Htemp: 0 < remset_gen_size h' from - n). {
+                unfold remset_gen_size. rewrite <- Heqgn, <- Heqrh_size. lia. }
+              assert (Hgesc2: general_enough_space_to_copy g2 h2 from to
+                                (remset_gen_size h' from - n)) by
+                (eapply forward_graph_and_heap_O_gestc; try eassumption; lia).
+              assert (Hulta: used_space (nth_space h2 to) < available_space (nth_space h2 to)). {
+                red in Hgesc2. pose proof unmarked_gen_size_nonneg g2 from.
+                unfold rest_gen_size in Hgesc2. lia. } clear Htemp Hgesc2.
+              sep_apply (heap_unused_rep_incr g2 h2 to). Intros.
+              gather_SEP (heap_struct_rep _ _ _) (heap_unused_rep _).
+              replace_SEP 0 (heap_rep sh (incr_remset_heap h2 (Z.of_nat to)) hp) by
+                (unfold heap_rep; entailer !!).
+              pose proof generation_share_writable (nth_gen g2 to) as Hws. rewrite Hsht2 in Hws.
+              gather_SEP (data_at_ _ _ _) (heap_remset_rep _ _ _). Intros.
+              assert (Hrhhc2: remset_heap_and_heap_compatible rh' h2). {
+                apply heap_relation_rhhc with h'; auto.
+                pose proof heaprel_forward_graph_and_heap from to O ft g' h'.
+                rewrite <- Hfgh in H. simpl in H. assumption. }
+              assert ((g2, incr_remset_heap h2 (Z.of_nat to),
+                        upd_remset_heap (RemSetInterior (InteriorVertexPos v pos)) rh' to,
+                        upd_remset from to g' (RemSetInterior (InteriorVertexPos v pos)) rmst') =
+                        forward_remset_item from to (g', h', rh', rmst')
+                          (RemSetInterior (InteriorVertexPos v pos))). {
+                simpl. rewrite <- Nat.eqb_neq in Hvnot. rewrite Hvnot. simpl. rewrite <- Heqft.
+                rewrite <- Hfgh. reflexivity. }
+              forward.
+              Exists g2 (incr_remset_heap h2 (Z.of_nat to))
+                (upd_remset_heap (RemSetInterior (InteriorVertexPos v pos)) rh' to)
+                (upd_remset from to g' (RemSetInterior (InteriorVertexPos v pos)) rmst').
+              unfold limit_address. clear Heqfp. rewrite <- Hgens in Haddrf'.
+              entailer !!. 1: rewrite Haddrf'; unfold available_size; f_equal. lia. simpl. cancel.
+              pose proof fr_forward_graph_and_heap from to 0
+                (field2forward (Znth pos (make_fields g' v))) g' h' as Hfr. rewrite <- Hfgh in Hfr.
+              simpl fst in Hfr. replace (vertex_address g' v) with (vertex_address g2 v).
+              2: { symmetry. eapply fr_vertex_address; eauto. apply graph_has_v_in_closure; assumption. }
+              sep_apply remset_rep_upd_int; auto.
+           ++ destruct vret as [Hvin | Hvnot]. 2: contradiction. subst P. clear Pweak Hweakp H. Intros.
+              sep_apply (graph_and_heap_rest_v_in_range_iff_offset g' h' from v pos). Intros.
+              rewrite <- Hgens, Heqfn, Heqgn, H in Hvin. forward. Exists g' h' rh' rmst'.
+              entailer !!.
+              ** split. 2: f_equal; lia. simpl. rewrite Nat.eqb_refl. simpl. reflexivity.
+              ** unfold heap_rep. cancel.
+           ++ Intros g3 h3 rh3 rmst3. rename H into Hfri. forward.
+              Exists (n + 1) g3 h3 rh3 rmst3.
+              pose proof fri_available_size _ _ _ _ _ _ _ _ _ _ _ Hftneq Hfri as Hfas.
+              pose proof fri_total_size _ _ _ _ _ _ _ _ _ _ _ Hftneq Hfri as Hfts.
+              assert (Hfss: space_start (nth_space h3 from) = space_start (nth_space h' from)). {
+                apply forward_remset_item_whr in Hfri. hnf in Hfri. destruct Hfri as [Hfri _].
+                rewrite Hfri. reflexivity. } rewrite Hfas, Hfts, Hfss.
+              assert (Hrheq: nth_remset_space rh from = nth_remset_space rh' from). {
+                eapply fri_fold_rh_same; eauto. pose proof gen_range_heap _ _ _ Hghc Hghgt.
+                clear -H Hrhhc. hnf in Hrhhc. rewrite Forall2_forall_Znth in Hrhhc. lia. }
+              entailer !!. split; [|split].
+              ** rewrite <- nth_remset_space_Znth in *.
+                 rewrite Hrheq in *. rewrite sublist_last_1 by lia.
+                 rewrite fold_left_app, <- Hfric. auto. rewrite <- Heqitem.
+                 Opaque forward_remset_item. simpl. Transparent forward_remset_item. assumption.
+              ** rewrite Hrhs, <- Hrheq in Hnrange. rewrite (rhhc_rssc_len g h rh) in Hnrange; auto. lia.
+              ** f_equal. simpl. unfold WORD_SIZE. lia.
+      * forward. Exists g' h' rh' rmst'. entailer !!. fold (remset_gen_size h from) in Hnrange.
+        rewrite <- Hrgseq in Hnrange. unfold remset_gen_size in Hnrange.
+        assert (Hn: n = total_size h' from - available_size h' from). {
+          clear -H Hnrange Hptrf'. remember (space_start (nth_space h' from)).
+          destruct v; try contradiction. simpl in H.
+          inversion H. rewrite !Ptrofs.Z_mod_modulus_eq in H1.
+          rewrite !(Z.add_comm (Ptrofs.unsigned i)) in H1. assert (Ptrofs.modulus > 0) by rep_lia.
+          apply Zmod_plus_inv in H1; auto. rewrite !Ptrofs.unsigned_repr_eq in H1.
+          rewrite <- (Z.add_0_r ((WORD_SIZE * (available_size h' from + n)) mod Ptrofs.modulus)) in H1.
+          rewrite <- (Z.add_0_r ((WORD_SIZE * (total_size h' from)) mod Ptrofs.modulus)) in H1.
+          rewrite !Z.add_mod_idemp_l in H1 by lia. rewrite !Z.add_0_r in H1.
+          pose proof total_space_unsigned_range (nth_space h' from). fold (total_size h' from) in H2.
+          rewrite !Z.mod_small in H1; [unfold WORD_SIZE in H1; lia | assumption |].
+          assert (0 <= available_size h' from + n <= total_size h' from). {
+            split. 2: lia. unfold available_size.
+            pose proof used_leq_available (nth_space h' from). lia. }
+          unfold WORD_SIZE in *; lia. } fold (remset_gen_size h' from) in Hn.
+        rewrite Hrgseq in Hn. erewrite compatible_remset_gen_size in Hn; eauto.
+        unfold forward_remset_gh. rewrite sublist_same in Hfric; easy.
+Qed.
+
+(* Print Assumptions body_forward_remset. *)
